src/FlatReturn.v
@@ -137,6 +137,27 @@ Definition SPlusCons := @StepLib.SPlusCons state.
 Require Import Metadata.
 Require Semantics.
 
+
+Definition prog_type : Type := env * list metadata.
+Definition valtype := unit.
+
+Inductive is_callstate (prog : prog_type) : valtype -> valtype -> state -> Prop :=.
+
+Inductive final_state (prog : prog_type) : state -> valtype -> Prop :=
+| FinalState : forall v, final_state prog (Stop v) tt.
+
+Definition initial_env (prog : prog_type) : env := fst prog.
+
+Definition semantics (prog : prog_type) : Semantics.semantics :=
+  @Semantics.Semantics_gen state env valtype
+                 (is_callstate prog)
+                 (sstep)
+                 (final_state prog)
+                 (initial_env prog).
+
+
+(*
+
 Definition prog_type : Type := env * list metadata.
 
 Inductive initial_state (prog : prog_type) : state -> Prop :=.
@@ -153,7 +174,7 @@ Definition semantics (prog : prog_type) : Semantics.semantics :=
                  (final_state prog)
                  (initial_env prog).
 
-
+*)
 
 (*
  * Mutual recursion/induction schemes for expr
