src/TaggedNumbered.v
@@ -1163,24 +1163,31 @@ Definition prog_type : Type := list expr * list metadata * list (list (expr * re
 
 Require Semantics.
 
+Definition valtype := unit. 
+
 Definition initial_env (prog : prog_type) : env := fst (fst (fst prog)).
 
-Inductive initial_state (prog : prog_type) : state -> Prop :=
-| init :
-    forall expr,
-      In expr (initial_env prog) ->
-      initial_state prog (Run expr nil (fun x => Stop x)).
+Inductive is_callstate (prog : prog_type) : valtype -> valtype -> state -> Prop := .
+(* TODO: stub *)
 
-Inductive final_state (prog : prog_type) : state -> Prop :=
+
+(* Inductive initial_state (prog : prog_type) : state -> Prop := *)
+(* | init : *)
+(*     forall expr, *)
+(*       In expr (initial_env prog) -> *)
+(*       initial_state prog (Run expr nil (fun x => Stop x)). *)
+
+Inductive final_state (prog : prog_type) : state -> valtype -> Prop :=
 | fine :
     forall expr,
       value expr ->
-      final_state prog (Stop expr).
+      final_state prog (Stop expr) tt.
 
 Definition semantics (prog : prog_type) : Semantics.semantics :=
-  @Semantics.Semantics_gen state env
+  @Semantics.Semantics_gen state env valtype
+                 (is_callstate prog)
                  (sstep)
-                 (initial_state prog)
+                 (* (initial_state prog) *)
                  (final_state prog)
                  (initial_env prog).
 
