src/FmajorComp.v
@@ -1066,7 +1066,8 @@ Qed.
     - apply well_founded_ltof.
     - inversion 1. (* TODO - replace with callstate matching *)
     - intro. intros0 II Afinal.
-      invc Afinal. invc II. on >I, invc. on >I_cont, invc. eexists. constructor.
+      invc Afinal. invc II. on >I, invc. on >I_cont, invc. eexists. split. constructor.
+      admit.
     - intros0 Astep. intros0 II.
       eapply raw_sim_lockstep; eauto. simpl.
       eapply I'_sim; try eassumption.
