src/OeufProof.v
@@ -53,26 +53,29 @@ Require Import EricTact.
 Section Simulation.
 
   Variable prog : compilation_unit.
-  Variable tprog : Asm.program.
-  Hypothesis TRANSF : transf_to_asm prog = OK tprog.
+  Variable tprog : Cminor.program.
+  Hypothesis TRANSF : transf_to_cminor prog = OK tprog.
 
   (* In this theorem we grab all of the things we need from all of the passes *)
   Theorem Oeuf_forward_simulation :
     forall ty,
-      mix_forward_simulation (@CompilationUnit.source_semantics ty prog) (Asm_semantics tprog).
+      mix_forward_simulation (@CompilationUnit.source_semantics ty prog) (Cminor_semantics tprog).
   Proof.
     (* SourceLang to Untyped *)
-    unfold transf_to_asm in TRANSF.
+    unfold transf_to_cminor in TRANSF.
     unfold OeufCompcertCompiler.apply_partial in *.
     break_match_hyp; try congruence.
     simpl in Heqr. inversion Heqr. clear Heqr.
     intro.
     eapply compose_notrace_mix_forward_simulation.
     eapply UntypedComp.fsim; try eassumption.
-
+    repeat (break_match_hyp; try congruence); try solve [inv H0].
+    inv H0. reflexivity.
+    
+    repeat (break_match_hyp; try congruence); try solve [inv H0].
+    inv H0. 
 
     (* Break down structure of compiler *)
-    unfold transf_untyped_to_asm in *.
     unfold transf_untyped_to_cminor in *.
     unfold OeufCompcertCompiler.apply_partial in *.
     unfold OeufCompcertCompiler.apply_total in *.
@@ -80,9 +83,13 @@ Section Simulation.
     repeat (break_match_hyp; try congruence).
     break_result_chain.
 
+    
     (* Untyped to Lifted *)
     eapply compose_notrace_mix_forward_simulation.
-    eapply LiftedComp.fsim; solve [eauto].
+    eapply LiftedComp.fsim; try solve [eauto].
+    unfold Metadata.check_length. simpl.
+    rewrite e. break_match; try congruence.
+    reflexivity.
     
     (* Lifted to Tagged *)
     eapply compose_notrace_mix_forward_simulation.
@@ -160,13 +167,9 @@ Section Simulation.
     admit. admit.
 
     (* Cmajor to Cminor *)
-    eapply TraceSemantics.compose_forward_simulation.
     eapply Cmajortominor.fsim; try eassumption.
-
-    (* Cminor to Asm *)
-    eapply OeufCompcertSimulations.transf_cminor_program_correct.
-    rewrite print_identity in *. subst p0.    
-    eassumption.
+    rewrite OeufCompcertCompiler.print_identity in *.
+    congruence.
     
   Admitted.
 
@@ -176,6 +179,7 @@ Section Simulation.
   (* Top level match states: we will write by hand, and make an easier definition to read *)
   Inductive match_states {ty} (expr : SourceLang.expr nil ty) (st : Asm.state) : Prop :=.
 
+  (*
   Lemma match_states_equiv :
     forall {ty} expr st,
       match_states expr st <-> (exists i, Oeuf_forward_simulation ty i expr st).
@@ -202,7 +206,8 @@ Section Simulation.
     admit.
     eapply match_states_equiv; eauto.
   Admitted.
-
+   *)
+  (*
   Theorem final_states_match :
     forall {ty} (expr : SourceLang.expr nil ty) st,
       SourceLang.value expr ->
@@ -212,7 +217,8 @@ Section Simulation.
   Proof.
     (* TODO: make r not an int, but a pointer. *)
   Admitted.
-
+*)
+(*
   Theorem final_state_nostep :
     forall st r,
       Asm.final_state st r ->
@@ -223,11 +229,13 @@ Section Simulation.
     clear HeqH2.
     inv H2. eauto.
   Qed.
-
+ *)
+  (*
   Definition match_initial_states_field {ty} := (MixSemantics.fsim_match_initial_states (source_semantics prog) (Asm_semantics tprog) (Oeuf_forward_simulation ty)).
-
+*)
   (* Here's how we show that we establish matching for initial symbols in our program *)
   (* i.e. what we call to build closures *)
+  (*
   Theorem match_initial_states :
     forall ty expr,
       CompilationUnit.initial_state prog nil ty expr ->
@@ -241,7 +249,7 @@ Section Simulation.
     rewrite <- match_states_equiv in H1.
     eauto.
   Qed.
-
+*)
 
   Definition compose_states (st1 st2 : Asm.state) : Asm.state :=
     (* TODO write this function  *)
